WIP for more general adequacy theorem

theories/Iris/BinaryAdequacy.v
@@ -128,29 +128,29 @@ Module Type IrisAdequacy2
     - clear s1. solve_inG.
  Qed.
 
-(*   Lemma steps_to_erased {σ Γ γ μ δ} (s : Stm Γ σ) {γ' μ' δ' s'}: *)
-(*     ⟨ γ, μ, δ, s ⟩ --->* ⟨ γ', μ', δ', s' ⟩ -> *)
-(*     rtc erased_step ([MkConf s δ]%list, (γ,μ)) ([MkConf s' δ']%list, (γ',μ')). *)
-(*   Proof. *)
-(*     induction 1; first done. *)
-(*     refine (rtc_l _ _ _ _ _ IHSteps). *)
-(*     exists nil. *)
-(*     refine (step_atomic _ _ _ _ _ nil nil eq_refl eq_refl _). *)
-(*     by eapply mk_prim_step. *)
-(*   Qed. *)
+  Lemma steps_to_erased {σ Γ γ μ δ} (s : Stm Γ σ) {γ' μ' δ' s'}:
+    ⟨ γ, μ, δ, s ⟩ --->* ⟨ γ', μ', δ', s' ⟩ ->
+    rtc erased_step ([MkConf s δ]%list, (γ,μ)) ([MkConf s' δ']%list, (γ',μ')).
+  Proof.
+    induction 1; first done.
+    refine (rtc_l _ _ _ _ _ IHSteps).
+    exists nil.
+    refine (step_atomic _ _ _ _ _ nil nil eq_refl eq_refl _).
+    by eapply mk_prim_step.
+  Qed.
 
-(*   Lemma steps_to_nsteps {σ Γ γ μ δ} (s : Stm Γ σ) {γ' μ' δ' s'}: *)
-(*     ⟨ γ, μ, δ, s ⟩ --->* ⟨ γ', μ', δ', s' ⟩ -> *)
-(*     exists n, language.nsteps n ([MkConf s δ]%list , (γ,μ)) [] ([MkConf s' δ']%list , (γ',μ')). *)
-(*   Proof. *)
-(*     induction 1. *)
-(*     - exists 0. now constructor. *)
-(*     - destruct IHSteps as [n steps]. *)
-(*       exists (S n). *)
-(*       refine (language.nsteps_l _ _ _ _ [] _ _ steps). *)
-(*       refine (step_atomic _ _ _ _ _ nil nil eq_refl eq_refl _). *)
-(*       now eapply mk_prim_step. *)
-(*   Qed. *)
+  Lemma steps_to_nsteps {σ Γ γ μ δ} (s : Stm Γ σ) {γ' μ' δ' s'}:
+    ⟨ γ, μ, δ, s ⟩ --->* ⟨ γ', μ', δ', s' ⟩ ->
+    exists n, language.nsteps n ([MkConf s δ]%list , (γ,μ)) [] ([MkConf s' δ']%list , (γ',μ')).
+  Proof.
+    induction 1.
+    - exists 0. now constructor.
+    - destruct IHSteps as [n steps].
+      exists (S n).
+      refine (language.nsteps_l _ _ _ _ [] _ _ steps).
+      refine (step_atomic _ _ _ _ _ nil nil eq_refl eq_refl _).
+      now eapply mk_prim_step.
+  Qed.
 
   Lemma own_RegStore_to_map_reg_pointsTos `{sailGS2 Σ} {γ1 γ2 : RegStore} {l : list (sigT 𝑹𝑬𝑮)} :
     NoDup l ->
@@ -201,14 +201,6 @@ Module Type IrisAdequacy2
   | nstep_trans {n} {γ2 γ3 : RegStore} {μ2 μ3 : Memory} {δ2 δ3 : CStore Γ} {s2 s3 : Stm Γ σ} :
       Step γ1 μ1 δ1 γ2 μ2 δ2 s1 s2 -> NSteps γ2 μ2 δ2 s2 γ3 μ3 δ3 s3 n -> NSteps γ1 μ1 δ1 s1 γ3 μ3 δ3 s3 (S n).
 
-  Lemma steps_to_nsteps {Γ : PCtx} {σ : Ty} {γ1 γ2 : RegStore} {μ1 μ2 : Memory} {δ1 δ2 : CStore Γ} {s1 s2 : Stm Γ σ} :
-    Steps γ1 μ1 δ1 s1 γ2 μ2 δ2 s2 -> exists n, NSteps γ1 μ1 δ1 s1 γ2 μ2 δ2 s2 n.
-  Proof.
-    induction 1 as [|γ1 μ1 δ1 s1 γ2 γ3 μ2 μ3 δ2 δ3 s2 s3 eval evals [n nsteps]].
-    - exists 0. constructor.
-    - exists (S n). econstructor; eassumption.
-  Qed.
-
   Lemma nsteps_to_steps {Γ : PCtx} {σ : Ty} {γ1 γ2 : RegStore} {μ1 μ2 : Memory} {δ1 δ2 : CStore Γ} {s1 s2 : Stm Γ σ} {n} :
     NSteps γ1 μ1 δ1 s1 γ2 μ2 δ2 s2 n -> Steps γ1 μ1 δ1 s1 γ2 μ2 δ2 s2.
   Proof.
@@ -236,17 +228,192 @@ Module Type IrisAdequacy2
     by apply Hprogress.
   Qed.
 
-  (* Lemma adequacy {Γ τ} (s1 s2 : Stm Γ τ) *)
-  (*   {γ11 γ12 γ21 γ22 : RegStore} {μ11 μ12 μ21 μ22 : Memory} *)
-  (*   {δ1 δ2 : CStore Γ} *)
-  (*   {Q : Val τ -> Prop} : *)
-  (*   ⟨ γ11, μ11, δ1, s1 ⟩ --->* ⟨ γ12, μ12, δ2, s2 ⟩ -> *)
-  (*   ⟨ γ21, μ21, δ1, s1 ⟩ --->* ⟨ γ22, μ22, δ2, s2 ⟩ -> *)
-  (*   Final s2 -> *)
-  (*   (forall `{sailGS2 Σ}, *)
-  (*       ⊢ semTriple δ1 (mem_res2 μ11 μ21 ∗ own_regstore2 γ11 γ21) s1 (fun v _ => ⌜Q v⌝)) -> *)
-  (*   ResultOrFail s2 Q. *)
-  (* Admitted. *)
+  Lemma not_stuck_ever {Γ τ} :
+    ∀ (e : expr (microsail_lang Γ τ)) σ,
+      not_stuck e σ.
+  Proof.
+    intros [s δ] [γ μ]. unfold not_stuck. cbn. destruct (stm_to_val s) eqn:Es.
+    - left. auto.
+    - right. apply reducible_not_val. auto.
+  Qed.
+
+  Definition ResultOrFail2 {Γ1 Γ2 τ} (s1 : Stm Γ1 τ) (s2 : Stm Γ2 τ) :
+    (Val τ -> Prop) -> Prop :=
+    match s1, s2 with
+    | stm_val _ v1, stm_val _ v2 => λ POST, v1 = v2 ∧ POST v1
+    | stm_fail _ m1, stm_fail _ m2 => λ _, True
+    | _, _ => λ _, False
+    end.
+
+  (* TODO: give this some more thought. Feels icky that the RHS doesn't play
+           a role in deriving φ. Another question is why we generalize over
+           a postcond Q, it doesn't relate to φ in any way?
+           Definitely check out how this is done in ReLoC. *)
+  Lemma wp2_adequacy {Γ1 Γ2 τ} (s1 s1' : Stm Γ1 τ) (s2 s2' : Stm Γ2 τ)
+    {γ1 γ1' γ2 γ2' : RegStore} {μ1 μ1' μ2 μ2' : Memory}
+    {δ1 δ1' : CStore Γ1} {δ2 δ2' : CStore Γ2}
+    {Q : ∀ `{sailGS2 Σ}, IVal τ -> CStore Γ1 -> IVal τ -> CStore Γ2 -> iProp Σ}
+    {φ : Prop} :
+    ⟨ γ1, μ1, δ1, s1 ⟩ --->* ⟨ γ1', μ1', δ1', s1' ⟩ ->
+    (* ⟨ γ2, μ2, δ2, s2 ⟩ --->* ⟨ γ2', μ2', δ2', s2' ⟩ -> *)
+    (* semWP2 already gives the above hypo, don't need it here (wrong res) *)
+    (forall `{sailGS2 Σ},
+        mem_res2 μ1 μ2 ∗ own_regstore2 γ1 γ2
+          ⊢ semWP2 δ1 δ2 s1 s2 Q ∗ (mem_inv(*2*) (mG := memGS2_memGS_left)  μ1' (*μ2'*) ={⊤,∅}=∗ ⌜φ⌝))%I ->
+    (* Just mem_inv should be enough, for the RHS, it is part of semWP2, so
+       this should be okay. *)
+    φ.
+  Proof.
+    intros [n1 steps1]%steps_to_nsteps (* Hs2 *) H.
+    refine (wp_strong_adequacy sailΣ2 (microsail_lang Γ1 τ) _ _ _ _ _ _ _ _ (fun _ => 0) _ steps1).
+    iIntros (Hinv).
+    assert (regsmapv1 := RegStore_to_map_valid γ1).
+    assert (regsmapv2 := RegStore_to_map_valid γ2).
+    iMod (own_alloc ((● RegStore_to_map γ1 ⋅ ◯ RegStore_to_map γ1 ) : regUR)) as (spec_name1) "[H1γ1 H2γ1]";
+      first by apply auth_both_valid.
+    iMod (own_alloc ((● RegStore_to_map γ2 ⋅ ◯ RegStore_to_map γ2 ) : regUR)) as (spec_name2) "[H1γ2 H2γ2]";
+      first by apply auth_both_valid.
+    pose proof (memΣ_GpreS2 (Σ := sailΣ2) _) as mGS.
+    iMod (mem_inv_init2 (mGS := mGS) μ1 μ2) as (memG) "[Hmem Rmem]".
+    set (regsG_left := {| reg_inG := @reg_pre_inG2_left sailΣ2 (@subG_sailGpreS sailΣ2 (subG_refl sailΣ2)); reg_gv_name := spec_name1 |}).
+    set (regsG_right := {| reg_inG := @reg_pre_inG2_right sailΣ2 (@subG_sailGpreS sailΣ2 (subG_refl sailΣ2)); reg_gv_name := spec_name2 |}).
+    set (sailG_left  := SailGS Hinv regsG_left  (@memGS2_memGS_left _ memG)).
+    set (sailG_right := SailGS Hinv regsG_right (@memGS2_memGS_right _ memG)).
+    set (gs2 := SailGS2 Hinv (SailRegGS2 (@sailGS_sailRegGS _ sailG_left) (@sailGS_sailRegGS _ sailG_right)) memG).
+    iModIntro.
+    iExists (λ σ _ _ _, regs_inv (srGS := regsG_left) (σ.1) ∗ @mem_inv _ (@memGS2_memGS_left _ memG) (σ.2))%I.
+    iExists [_]%list, _, _. cbn.
+    rewrite mem_inv2_mem_inv. iDestruct "Hmem" as "($ & Hmem)".
+    iSplitL "H1γ1".
+    { now iApply (@own_RegStore_to_regs_inv _ regsG_left γ1). }
+    iPoseProof (H _ gs2 with "[$Rmem H2γ1 H2γ2]") as "(H & HΦ)".
+    { iApply (own_RegStore_to_map_reg_pointsTos (l := finite.enum (sigT 𝑹𝑬𝑮))).
+      eapply finite.NoDup_enum. iFrame "H2γ1". iApply "H2γ2". }
+    rewrite /semWP2 /semWP.
+    iDestruct ("H" with "[H1γ2 $Hmem]") as "$".
+    { now iApply own_RegStore_to_regs_inv. }
+    iIntros (es' t2') "_ _ _ [Hregs Hmem] _ _".
+    now iApply "HΦ".
+    (* iIntros (es' t2') "%Happ %Hlen %Hns [Hregs Hmem] H _". *)
+    (* destruct es'; try discriminate. *)
+    (* inversion Happ; subst. simpl. *)
+    (* iDestruct "H" as "(H & _)". *)
+    (* specialize (Hns (MkConf s1' δ1') eq_refl (elem_of_list_here _ _)). *)
+    (* destruct Hns as [Hns|Hns]. *)
+    (* - cbn in Hns. destruct Hns as [(v1' & δ1'') Hns]. rewrite Hns. simpl. *)
+    (*   iDestruct "H" as "(% & % & % & % & % & ? & ? & ? & Hmem22 & ?)". *)
+    (*   iApply "HΦ". *)
+  Qed.
+
+
+  Lemma wp2_adequacy' {Γ1 Γ2 τ} (s1 : Stm Γ1 τ) (s2 : Stm Γ2 τ)
+    {γ1 γ2 : RegStore} {μ1 μ2 : Memory}
+    {δ1 : CStore Γ1} {δ2 : CStore Γ2}
+    {Q : IVal τ -> CStore Γ1 -> IVal τ -> CStore Γ2 -> Prop} :
+    (forall `{sailGS2 Σ},
+        ⊢ mem_res2 μ1 μ2 ∗ own_regstore2 γ1 γ2 -∗ semWP2 δ1 δ2 s1 s2 (λ v1 δ1 v2 δ2, ⌜Q v1 δ1 v2 δ2⌝)) ->
+    adequate NotStuck (MkConf s1 δ1) (γ1, μ1)
+      (λ v1 _, ∃ s2' δ2' γ2' μ2', rtc erased_step ([MkConf s2 δ2]%list, (γ2, μ2)) ([MkConf s2' δ2']%list, (γ2', μ2')) ∧ Final s2' ∧ match s2' with
+                                                                                                                                    | stm_val _ v2 => Q (valconf_val v1) (valconf_store v1) (inl v2) δ2'
+                                                                                                                                    | stm_fail _ m2 => Q (valconf_val v1) (valconf_store v1) (inr m2) δ2'
+                                                                                                                                    | _ => False
+                                                                                                                                    end).
+  Proof.
+    intros wp2.
+    apply (wp_adequacy sailΣ2 (microsail_lang Γ1 τ) NotStuck (MkConf s1 δ1) (γ1, μ1)).
+    iIntros (Hinv κs).
+    assert (regsmapv1 := RegStore_to_map_valid γ1).
+    assert (regsmapv2 := RegStore_to_map_valid γ2).
+    iMod (own_alloc ((● RegStore_to_map γ1 ⋅ ◯ RegStore_to_map γ1 ) : regUR)) as (spec_name1) "[H1γ1 H2γ1]";
+      first by apply auth_both_valid.
+    iMod (own_alloc ((● RegStore_to_map γ2 ⋅ ◯ RegStore_to_map γ2 ) : regUR)) as (spec_name2) "[H1γ2 H2γ2]";
+      first by apply auth_both_valid.
+    pose proof (memΣ_GpreS2 (Σ := sailΣ2) _) as mGS.
+    iMod (mem_inv_init2 (mGS := mGS) μ1 μ2) as (memG) "[Hmem Rmem]".
+    set (regsG_left := {| reg_inG := @reg_pre_inG2_left sailΣ2 (@subG_sailGpreS sailΣ2 (subG_refl sailΣ2)); reg_gv_name := spec_name1 |}).
+    set (regsG_right := {| reg_inG := @reg_pre_inG2_right sailΣ2 (@subG_sailGpreS sailΣ2 (subG_refl sailΣ2)); reg_gv_name := spec_name2 |}).
+    set (sailG_left  := SailGS Hinv regsG_left  (@memGS2_memGS_left _ memG)).
+    set (sailG_right := SailGS Hinv regsG_right (@memGS2_memGS_right _ memG)).
+    set (gs2 := SailGS2 Hinv (SailRegGS2 (@sailGS_sailRegGS _ sailG_left) (@sailGS_sailRegGS _ sailG_right)) memG).
+    iModIntro.
+    iExists (fun σ _ => regs_inv (srGS := regsG_left) (σ.1) ∗ @mem_inv _ (@memGS2_memGS_left _ memG) (σ.2))%I.
+    iExists _.
+    rewrite mem_inv2_mem_inv. cbn. iDestruct "Hmem" as "($ & Hmem)".
+    iSplitL "H1γ1".
+    { now iApply (@own_RegStore_to_regs_inv _ regsG_left γ1). }
+    iPoseProof (wp2 _ gs2 with "[$Rmem H2γ1 H2γ2]") as "H".
+    { iApply (own_RegStore_to_map_reg_pointsTos (l := finite.enum (sigT 𝑹𝑬𝑮))).
+      eapply finite.NoDup_enum.
+      iSplitL "H2γ1". iApply "H2γ1". iApply "H2γ2". }
+    rewrite /semWP2 /semWP.
+    iSpecialize ("H" with "[H1γ2 $Hmem]").
+    { now iApply own_RegStore_to_regs_inv. }
+    iApply (wp_mono with "H").
+    iIntros (v1) "(%γ2' & %μ2' & %δ2' & %s2' & %v2 & %Hstep & %Heq & Hreg & Hmem & %HQ)".
+    iExists s2', δ2', γ2', μ2'. destruct v1 as [[v1|m1] δ1']; simpl in *;
+      iPureIntro; repeat split.
+    - now apply steps_to_erased.
+    - apply (stm_to_val_Final Heq).
+    - destruct (stm_to_val_Some_cases Heq) as [(v' & -> & ->)|(m' & -> & ->)]; auto.
+    - now apply steps_to_erased.
+    - apply (stm_to_val_Final Heq).
+    - destruct (stm_to_val_Some_cases Heq) as [(v' & -> & ->)|(m' & -> & ->)]; auto.
+  Qed.
+
+  (* NOTE: more general stmt, generalized over diff programs (in terms of the actual program logic, instead of the semTriple) *)
+  Lemma adequacy {Γ τ} (s : Stm Γ τ)
+    {γ1 γ2 : RegStore} {μ1 μ2 : Memory}
+    {δ : CStore Γ}
+    {Q : Val τ -> Prop} :
+    (forall `{sailGS2 Σ},
+        ⊢ semTriple δ (mem_res2 μ1 μ2 ∗ own_regstore2 γ1 γ2) s (fun v _ => ⌜Q v⌝)) ->
+    adequate NotStuck (MkConf s δ) (γ1, μ1)
+             (λ v _, ∃ s' δ' γ2' μ2', rtc erased_step ([MkConf s δ]%list, (γ2, μ2)) ([MkConf s' δ']%list, (γ2', μ2')) ∧ Final s' ∧ @ResultOrFail2 Γ _ _ (of_ival (valconf_val v)) s' Q).
+  Proof.
+    intros trips.
+    apply (wp_adequacy sailΣ2 (microsail_lang Γ τ) NotStuck (MkConf s δ) (γ1, μ1)).
+    iIntros (Hinv κs).
+    assert (regsmapv1 := RegStore_to_map_valid γ1).
+    assert (regsmapv2 := RegStore_to_map_valid γ2).
+    iMod (own_alloc ((● RegStore_to_map γ1 ⋅ ◯ RegStore_to_map γ1 ) : regUR)) as (spec_name1) "[H1γ1 H2γ1]";
+      first by apply auth_both_valid.
+    iMod (own_alloc ((● RegStore_to_map γ2 ⋅ ◯ RegStore_to_map γ2 ) : regUR)) as (spec_name2) "[H1γ2 H2γ2]";
+      first by apply auth_both_valid.
+    pose proof (memΣ_GpreS2 (Σ := sailΣ2) _) as mGS.
+    iMod (mem_inv_init2 (mGS := mGS) μ1 μ2) as (memG) "[Hmem Rmem]".
+    set (regsG_left := {| reg_inG := @reg_pre_inG2_left sailΣ2 (@subG_sailGpreS sailΣ2 (subG_refl sailΣ2)); reg_gv_name := spec_name1 |}).
+    set (regsG_right := {| reg_inG := @reg_pre_inG2_right sailΣ2 (@subG_sailGpreS sailΣ2 (subG_refl sailΣ2)); reg_gv_name := spec_name2 |}).
+    set (sailG_left  := SailGS Hinv regsG_left  (@memGS2_memGS_left _ memG)).
+    set (sailG_right := SailGS Hinv regsG_right (@memGS2_memGS_right _ memG)).
+    set (gs2 := SailGS2 Hinv (SailRegGS2 (@sailGS_sailRegGS _ sailG_left) (@sailGS_sailRegGS _ sailG_right)) memG).
+    iModIntro.
+    iExists (fun σ _ => regs_inv (srGS := regsG_left) (σ.1) ∗ @mem_inv _ (@memGS2_memGS_left _ memG) (σ.2))%I.
+    iExists _.
+    rewrite mem_inv2_mem_inv. cbn. iDestruct "Hmem" as "($ & Hmem)".
+    iSplitL "H1γ1".
+    { now iApply (@own_RegStore_to_regs_inv _ regsG_left γ1). }
+    iPoseProof (trips _ gs2 with "[$Rmem H2γ1 H2γ2]") as "H".
+    { iApply (own_RegStore_to_map_reg_pointsTos (l := finite.enum (sigT 𝑹𝑬𝑮))).
+      eapply finite.NoDup_enum.
+      iSplitL "H2γ1". iApply "H2γ1". iApply "H2γ2". }
+    rewrite /semWP2 /semWP.
+    iSpecialize ("H" with "[H1γ2 $Hmem]").
+    { now iApply own_RegStore_to_regs_inv. }
+    iApply (wp_mono with "H").
+    iIntros (v1) "(%γ2' & %μ2' & %δ2' & %s2' & %v2 & %Hstep & %Heq & Hreg & Hmem & %Hvaleq & %Hstoreeq & H)".
+    iExists s2', δ2', γ2', μ2'. destruct v1 as [[v1|m1] δ1']; simpl in *;
+      iDestruct "H" as "%H"; iPureIntro; repeat split.
+    - now apply steps_to_erased.
+    - apply (stm_to_val_Final Heq).
+    - destruct (stm_to_val_Some_cases Heq) as [(v' & -> & ->)|(m' & -> & ->)].
+      + inversion Hvaleq; subst; auto.
+      + discriminate.
+    - now apply steps_to_erased.
+    - apply (stm_to_val_Final Heq).
+    - destruct (stm_to_val_Some_cases Heq) as [(v' & -> & ->)|(m' & -> & ->)].
+      + discriminate.
+      + inversion Hvaleq; subst; auto.
+  Qed.
 
   (* Lemma adequacy_gen {Γ1 Γ2 τ} (s11 s12 : Stm Γ1 τ) (s21 s22 : Stm Γ2 τ) *)
   (*   {γ11 γ12 γ21 γ22 : RegStore} {μ11 μ12 μ21 μ22 : Memory} *)
